# ABC convection-reaction equations

## Dimensional equations

strong form of the initial boundary value problem

$$
\begin{align*}
&\text{Find} \\
&\text{$a(\textbf{x}, t): \Omega\times[0, \infty) \to \mathbb{R}$, } \\
&\text{$b(\textbf{x}, t): \Omega\times[0, \infty) \to \mathbb{R}$, } \\
&\text{$c(\textbf{x}, t): \Omega\times[0, \infty) \to \mathbb{R}$, } \\
&\text{$\textbf{u}(\textbf{x}, t): \Omega\times[0, \infty) \to \mathbb{R}^d$ and $p(\textbf{x}, t): \Omega\times[0, \infty) \to \mathbb{R}$} \\
&\text{such that} \\
&\begin{cases}
\phi\frac{\partial a}{\partial t} + \textbf{u}\cdot\nabla a = \nabla\cdot(\mathsf{D}_a(\phi, \textbf{u})\cdot \nabla a) - R(a,b) \\
\phi\frac{\partial b}{\partial t} + \textbf{u}\cdot\nabla b = \nabla\cdot(\mathsf{D}_b(\phi, \textbf{u})\cdot \nabla b) - R(a,b) \\
\phi\frac{\partial c}{\partial t} + \textbf{u}\cdot\nabla c = \nabla\cdot(\mathsf{D}_c(\phi, \textbf{u})\cdot \nabla c) + R(a,b) \\
\nabla\cdot\textbf{u}=0 \\
\textbf{u}=-\frac{\mathsf{K}(\phi)}{\mu(a,b,c)}\cdot\left(\nabla p + \rho(a,b,c)g\,\textbf{e}_g\right) & \forall(\textbf{x}, t)\in\Omega\times[0,\infty)\\
a(\textbf{x},t=0)=a_0 \\
b(\textbf{x},t=0)=b_0 \\
c(\textbf{x},t=0)=c_0 \\
w = w_{\text{D},w} & \forall(\textbf{x}, t)\in\partial\Omega_{\text{D},w} \times [0,\infty]\quad\forall w\in\{a, b, c\}\\
\textbf{n}\cdot(\mathsf{D}_w\nabla w) = w_{\text{N}, w} & \forall(\textbf{x}, t)\in\partial\Omega_{\text{N},w} \times [0,\infty]\quad\forall w\in\{a, b, c\}\\
\textbf{n}\cdot\textbf{u} = u_{\text{E}} & \forall(\textbf{x}, t)\in\partial\Omega_{\text{E}} \times [0,\infty] \\
p = p_{\text{N}} & \forall(\textbf{x}, t)\in\partial\Omega_{\text{N}}\times [0,\infty]~,~\partial\Omega_{\text{N}}=\partial\Omega/\partial\Omega_{\text{E}}
\end{cases}~.
\end{align*}
$$

## Non-dimensional equations

$$
\begin{cases}
\phi\frac{\partial a}{\partial t} + Ad\,\textbf{u}\cdot\nabla a = \frac{1}{Pe}\nabla\cdot(\mathsf{D}_a(\phi, \textbf{u})\cdot \nabla a) - Ki R(a,b) \\
\phi\frac{\partial b}{\partial t} + Ad\,\textbf{u}\cdot\nabla b = \frac{1}{Le_bPe}\nabla\cdot(\mathsf{D}_b(\phi, \textbf{u})\cdot \nabla b) - Ki R(a,b) \\
\phi\frac{\partial c}{\partial t} + Ad\,\textbf{u}\cdot\nabla c = \frac{1}{Le_cPe}\nabla\cdot(\mathsf{D}_c(\phi, \textbf{u})\cdot \nabla c) + Ki R(a,b) \\
\nabla\cdot\textbf{u}=0 \\
\textbf{u}=-\frac{\mathsf{K}(\phi)}{\mu(a,b,c)}\cdot\left(\nabla p + Bu\,\rho(a,b,c)g\,\textbf{e}_g\right) \\
\end{cases}
$$

$$
\begin{align*}
Ad&=\frac{\mathcal{U}\mathcal{T}}{\phi_{\text{ref}}\mathcal{L}} \\
Pe&=\frac{\phi_{\text{ref}}\mathcal{L}^2}{D_{\text{ref}}\mathcal{T}} \\
Ki&=\frac{\mathcal{T}\Delta R}{\phi_{\text{ref}}\Delta c} \\
Bu&=\frac{K_{\text{ref}}\,g\Delta\rho}{\mu_{\text{ref}}\,\mathcal{U}} \\
\end{align*} 
$$